Safety and Correctness Fromalization Draft

Examples/p32_cfi.v
@@ -7,34 +7,57 @@ Require Import List.
 Open Scope N.
 Import ListNotations.
 
-(* id - label for the instruction
-   oid - label to check for with dynamic jumps
-   n - instruction encoding
-   a - instruction address *)
-Inductive inst_data := Data (id: option N) (oid: N) (n: N) (a: N).
+Definition id := N.
 
-(* add a label check to a jmpr instruction where the destination is rs1 *)
+(* iid - id for the instruction
+   oid - id to check for with dynamic jumps
+   n   - instruction encoding
+   a   - instruction address *)
+Inductive inst_data := Data (iid: option id) (oid: list id) (n: N) (a: N).
+
+(* generate code to check for each id in a list
+   ids - list of valid destination ids
+   r0  - register with the real id
+   r1  - scratch register to load constants into *)
+Fixpoint check_id_insts (ids: list id) (r0: N) (r1: N): list p32_asm :=
+  match ids with
+  | id::t => let tail := check_id_insts t r0 r1 in
+      [
+        PIL_li r1 id;                                    (* load next valid id *)
+        PIL_beq r0 r1 (4 + 4 * Z.of_nat (length tail))   (* if match, branch to the end *)
+      ] ++ tail                                          (* otherwise, check the rest of the ids *)
+  | nil => [PIL_beq 0 0 0]                               (* no valid ids, abort (infinite loop) *)
+  end.
+
+(* add an id check to a jmpr instruction
+   data - data of the jmpr instruction
+   rs1  - register that holds the destination *)
 Definition rewrite_jmpr (data: inst_data) (rs1: N) : list N :=
+  let r0 := if rs1 == 0 then 2 else 0 in
+  let r1 := if rs1 == 1 then 2 else 1 in
+  let sp := 6 in
   match data with Data _ oid _ _ =>
-    map assemble_insn [
-      PIL_st 0 6 0;       (*   st r0  sp  0 *) (* save r0 and r1 to the stack *)
-      PIL_st 1 6 4;       (*   st r1  sp  4 *)
-      PIL_ld 0 rs1 4;     (*   ld r0  rs1 4 *) (* load the real label and expected label *)
-      PIL_li 1 oid;       (*   li r1  oid   *)
-      PIL_bne 0 1 0;      (*  bne r0  r1  0 *) (* infinite loop if no match *)
-      PIL_ld 0 6 0;       (*   ld r0  sp  0 *) (* restore r0 and r1 *)
-      PIL_ld 1 6 4;       (*   ld r1  sp  4 *)
-      PIL_jmpr rs1        (* jmpr rs1       *) (* jump *)
-    ] end.
+    map assemble_insn ([
+      PIL_st   r0  sp  0;                (* save r0 and r1 to the stack *)
+      PIL_st   r1  sp  4;
+      PIL_ld   r0  rs1 4                 (* load the real id *)
+    ] ++ check_id_insts oid r0 r1 ++ [   (* compare against all valid id *)
+      PIL_ld   r0  sp  0;                (* restore r0 and r1 *)
+      PIL_ld   r1  sp  4;
+      PIL_jmpr rs1                       (* jump *)
+    ]) end.
 
-(* add a label at the start of a list of instructions *)
-Definition add_id (id: option N) (rw_n: list N) : list N :=
-  match id with
-  | Some id => assemble_insn (PIL_beq 0 0 8)::id::rw_n
+(* add a label to a rewritten instruction
+   i    - id of the instruction
+   rw_n - rewritten encoding of a single instruction *)
+Definition add_id (i: option id) (rw_n: list N) : list N :=
+  match i with
+  | Some i => assemble_insn (PIL_beq 0 0 8)::i::rw_n
   | None => rw_n
   end.
 
-(* rewrite a single instruction *)
+(* rewrite a single instruction
+   data - data of the instruction to rewrite *)
 Definition rewrite_inst (data: inst_data) : list N :=
   match data with Data id _ n _ =>
     let inst := p32_decode n in
@@ -45,39 +68,58 @@ Definition rewrite_inst (data: inst_data) : list N :=
     add_id id new_n
   end.
 
-(* get a list of the new starting addresses for each old instruction *)
+(* get a list of the new starting addresses for each old instruction
+   rw_ns - list of all rewritten instruction encodings
+   a     - base address *)
 Fixpoint new_addrs (rw_ns: list (list N)) (a: N) : list N :=
   match rw_ns with
   | n::ns => a::new_addrs ns (a + 4 * N.of_nat (length n))
-  | _ => a::nil
+  | _ => a::nil (* also add the address of the end of the program, so we can compute last_addrs easily *)
   end.
 
-(* get a list of the new destination addresses of jump/branch instructions *)
-Fixpoint new_targets (data: list inst_data) (rw_as: list N) (base: N) : list N :=
+(* get the immediate value of a jump/branch instruction
+   inst - the instruction *)
+Definition get_imm (inst: p32_asm) :=
+  match inst with
+  | PIL_beq rs1 rs2 si => si
+  | PIL_blt rs1 rs2 si => si
+  | PIL_bne rs1 rs2 si => si
+  | PIL_bl si => si
+  | PIL_jl i => Z.of_N i
+  | PIL_jmp i => Z.of_N i
+  | _ => 0%Z
+  end.
+
+(* get a list of the new destination addresses of jump/branch instructions in the original program
+   data      - data of the original program
+   new_addrs - new starting addresses of each instruction in the rewritten program
+   base      - base address of the program *)
+Fixpoint new_targets (data: list inst_data) (new_addrs: list N) (base: N) : list N :=
   match data with
   | Data _ _ n a::t => nth match p32_decode n with
-                           | PIL_beq rs1 rs2 si => (Z.to_nat ((Z.of_N a) + si) - N.to_nat base) / 4
-                           | PIL_blt rs1 rs2 si => (Z.to_nat ((Z.of_N a) + si) - N.to_nat base) / 4
-                           | PIL_bne rs1 rs2 si => (Z.to_nat ((Z.of_N a) + si) - N.to_nat base) / 4
-                           | PIL_bl si => (Z.to_nat ((Z.of_N a) + si) - N.to_nat base) / 4
-                           | PIL_jl i => (N.to_nat i - N.to_nat base) / 4
-                           | PIL_jmp i => (N.to_nat i - N.to_nat base) / 4
+                           | PIL_beq _ _ _ | PIL_blt _ _ _ | PIL_bne _ _ _ | PIL_bl _ => (Z.to_nat ((Z.of_N a) + get_imm (p32_decode n)) - N.to_nat base) / 4
+                           | PIL_jl _ | PIL_jmp _ => (Z.to_nat (get_imm (p32_decode n)) - N.to_nat base) / 4
                            | _ => 0
-                       end rw_as 0::new_targets t rw_as base
+                       end new_addrs 0::new_targets t new_addrs base
   | _ => nil
   end.
 
-(* change the destination of a direct jump/branch at addr a *)
-Definition replace_target (n: N) (a: N) (new_dest: N) : N :=
-    assemble_insn match p32_decode n with
-    | PIL_beq rs1 rs2 si => PIL_beq rs1 rs2 (Z.of_N new_dest - Z.of_N a)
-    | PIL_blt rs1 rs2 si => PIL_blt rs1 rs2 (Z.of_N new_dest - Z.of_N a)
-    | PIL_bne rs1 rs2 si => PIL_blt rs1 rs2 (Z.of_N new_dest - Z.of_N a)
-    | PIL_bl si => PIL_bl (Z.of_N new_dest - Z.of_N a)
-    | PIL_jl i => PIL_jl new_dest
-    | PIL_jmp i => PIL_jmp new_dest
-    | a => a
-  end.
+(* change the destination of a direct jump/branch, does nothing if a different instruction, returns None if the target is not reachable
+   n        - encoding of the instruction
+   a        - address of the instruction
+   new_dest - new address the instruction should go to *)
+Definition replace_target (n: N) (a: N) (new_dest: N) : option N :=
+  let new_inst := match p32_decode n with
+                  | PIL_beq rs1 rs2 si => PIL_beq rs1 rs2 (Z.of_N new_dest - Z.of_N a)
+                  | PIL_blt rs1 rs2 si => PIL_blt rs1 rs2 (Z.of_N new_dest - Z.of_N a)
+                  | PIL_bne rs1 rs2 si => PIL_blt rs1 rs2 (Z.of_N new_dest - Z.of_N a)
+                  | PIL_bl si => PIL_bl (Z.of_N new_dest - Z.of_N a)
+                  | PIL_jl i => PIL_jl new_dest
+                  | PIL_jmp i => PIL_jmp new_dest
+                  | a => a end in
+  let new_n := assemble_insn new_inst in
+  (* check if the immediate value is representable in the instruction encoding *)
+  if Z.eqb (get_imm (p32_decode new_n)) (get_imm new_inst) then Some new_n else None.
 
 (* replace the last element of a list *)
 Fixpoint replace_last {T: Type} (ts: list T) (last: T) : list T :=
@@ -87,29 +129,76 @@ Fixpoint replace_last {T: Type} (ts: list T) (last: T) : list T :=
   | nil => nil
   end.
 
-(* fix the destinations of the jump/branch instructions of a rewritten program *)
-Fixpoint fix_targets (ns: list N) (rw_as: list N) (rw_ts: list N) (rw_ns: list (list N)) : list (list N) :=
-  match ns, rw_as, rw_ts, rw_ns with
-  | n::ns, rw_a::rw_as, rw_t::rw_ts, rw_n::rw_ns =>
-      let new_last := (replace_target n (rw_a-4) rw_t) in
-      replace_last rw_n new_last::fix_targets ns rw_as rw_ts rw_ns
-  | _, _, _, _ => nil
+(* fix the destinations of the jump/branch instructions of a rewritten program, return None if an instruction could not be fixed
+   ns             - list of instruction encodings of the original program
+   last_addrs     - list of addresses of the last instruction of each rewritten instruction
+                      (we only need to fix the last instruction,
+                       since the rewriter only prepends instructions to each original instruction,
+                       and the inserted jumps/branches are already correct)
+   new_targets    - list of new targets for each original instruction (ignored if not a jump)
+   rewritten_prog - rewritten program to fix the jump targets of *)
+Fixpoint fix_targets (ns: list N) (last_addrs: list N) (new_targets: list N) (rewritten_prog: list (list N)) : option (list (list N)) :=
+  match ns, last_addrs, new_targets, rewritten_prog with
+  | n::ns, last_addr::last_addrs, new_target::new_targets, rewritten_n::rewritten_prog =>
+      let new_last := (replace_target n last_addr new_target) in
+      let rest := fix_targets ns last_addrs new_targets rewritten_prog in
+      match new_last, rest with
+      | Some new_last, Some rest => Some (replace_last rewritten_n new_last::rest)
+      | _, _ => None end
+  | _, _, _, _ => Some nil
   end.
 
-(* turn a list of inst encodings to a list of inst_data *)
-Fixpoint to_data (label: N -> option N) (Pol: N -> N) (ns: list N) (a: N) : list inst_data :=
+(* turn a list of inst encodings to a list of inst_data
+   label - instruction labeling
+   pol   - policy to enforce
+   ns    - list of instruction encodings
+   a     - starting address *)
+Fixpoint to_data (label: N -> option id) (pol: N -> list id) (ns: list N) (a: N) : list inst_data :=
   match ns with
-  | n::ns => (Data (label a) (Pol a) n a)::(to_data label Pol ns (a+4))
+  | n::ns => (Data (label a) (pol a) n a)::(to_data label pol ns (a+4))
   | nil => nil
   end.
 
-(* rewrite a program starting at address a *)
-Definition rewrite (label: N -> option N) (Pol: N -> N) (ns: list N) (a: N) : list (list N) :=
-  let data := to_data label Pol ns a in
-  let rw_ns := map rewrite_inst data in
-  let rw_as := new_addrs rw_ns a in
-  let rw_ts := new_targets data rw_as a in
-  fix_targets ns (tail rw_as) rw_ts rw_ns.
+(* rewrite a program
+   label - instruction labeling
+   pol   - policy to enforce
+   ns    - list of instruction encodings of the program
+   a     - starting address of the program *)
+Definition rewrite (label: N -> option id) (pol: N -> list id) (ns: list N) (a: N) : list (list N) :=
+  let data := to_data label pol ns a in
+  let rewritten_prog := map rewrite_inst data in
+  (* everything after is just to fix jump/branch targets from the original program *)
+  let new_addrs := new_addrs rewritten_prog a in
+  let new_targets := new_targets data new_addrs a in
+  let last_addrs := (map (fun a => a-4) (tail new_addrs)) in
+  match fix_targets ns last_addrs new_targets rewritten_prog with
+  | Some fixed => fixed
+  | None => nil
+  end.
+
+(* get all ids used in a labeling
+   label - instruction labeling
+   ns - original program encoding
+   a - starting address of the program *)
+Fixpoint all_ids (label: N -> option id) (ns: list N) (a: N) : list id :=
+  match ns, label a with
+  | n::t, Some id => id::all_ids label t (a+4)
+  | n::t, None => all_ids label t (a+4)
+  | nil, _ => nil
+  end.
+
+(* rewrite a program, but return nil if an id appears in the rewritten program where it shouldn't *)
+Definition rewrite_check_id (label: N -> option id) (pol: N -> list id) (ns: list N) (a: N)  :=
+  (* first, rewrite the program using a labeling only with Ns we already know appear in the rewritten program *)
+  let label' := (fun a => match label a with
+                          (* we know that this instruction will be added to the program *)
+                          | Some _ => Some (assemble_insn (PIL_beq 0 0 8))
+                          | _ => None end) in
+  let rw := concat (rewrite label' pol ns a) in
+  (* now check if any of the ids appear in the new program *)
+  let all_ids := all_ids label ns a in
+  let any_id_in_rw := existsb (fun id => existsb (fun n => N.eqb id n) rw) all_ids in
+  if any_id_in_rw then nil else rewrite label pol ns a.
 
 (*** simple test ***)
 
@@ -123,9 +212,9 @@ Definition my_label n :=
 
 Definition my_policy n :=
   match n with
-  | 0 => 111
-  | 12 => 222
-  | _ => 333
+  | 0 => [111]
+  | 12 => [222; 123; 232232323]
+  | _ => [333]
   end.
 
 Definition my_prog := (* random gibberish *)
@@ -145,3 +234,252 @@ Definition my_rewritten_prog := rewrite my_label my_policy my_prog 0.
 Compute my_prog.
 Compute my_rewritten_prog.
 Compute map (map p32_decode) my_rewritten_prog.
+
+(* This Section defines properties of rewriters with an aim of being general.
+   In other words, this should be reusable for rewriters implemented in different
+   ways. E.g. we define a Property of indices (N), `is_abort`, that is agnostic
+   to the definition of this property.
+
+   The safety property is formalized according to the email thread we had.
+
+   The other two properties, `rewritten_is_faithful` and `original_has_simulation`
+   are formalized according to the paper "Sound Transpilation from Binary␍
+   to Machine-Independent Code"  with signifcant differences from reasoning about
+   an assembly program that lives in the same address space as memory writes, 
+   rather than a BIL program.
+
+   Below, when we say 'executions' we mean an exeuction trace of an original binary
+   and its corresponding execution on the rewritten binary. *)
+Section RRCorrectness.
+  (* Parameters: |-- label  --|      |- policy -|     program  entry *)
+  Variable rr : (N -> option id) -> (N -> list id) -> list N -> N -> option (list (list N)).
+  Variable label : N -> option id.
+  Variables policy : N -> list id.
+  Variable program  : list N.
+  Variable entry : addr.
+  Variable program' : list (list N).
+  Variable is_abort : N -> Prop.
+  (* Added `is_aborted` as a trace Property for easy reading, but similar
+     name may be confusing. *)
+  Variable is_aborted : trace -> Prop.
+  (* For correctness we're reasoning over traces which operate at the
+     level of addresses* so we need to translate from an address to the 
+     corresponding index. 
+
+    * really `exits`, defined in Picinae_core.v, which can be exceptions,
+      but that's irrelevant here *)
+  Variable index_of_addr : addr -> option N.
+
+  (* Difine a similarity of states proposition that must hold between
+     the states of executions at the beginning of each block.
+
+     E.g. 
+     Definition similar_states s1 s2 : Prop :=
+        forall v, match v with
+        | R_R0 | R_R1 | R_R2 
+        | R_R3 | R_R4 | R_R5 
+        | R_SP | R_LR | R_PC => s1 v = s2 v
+        | _ => True
+        end.
+   *)
+  Variable similar_states : store -> store -> Prop.
+  Variables binary binary' : N.
+
+  (* find and return the length of the smallest prefix of r's output list whose 
+    list-flattened length equals or exceeds index.
+    Think of iindex n as the nth instruction in the flattened rrprog - instruction index,
+    The output is the number of blocks you need to take from rrprog the block with 
+      that instruction.
+    If the list is empty then the iindex is out of bounds... return 0 I guess... *)
+  Fixpoint block_index_impl (rrprog : list (list N)) (iindex : N) : N :=
+    match rrprog with
+    | [] => 0%N
+    | h :: t => 
+        (* Here the comparison is `Gt` because an n element list goes up to index n-1, not n *)
+        match N.compare (N.of_nat (length h)) iindex with
+        | Gt => 1
+        | _ =>  N.succ (block_index_impl t (iindex - (N.of_nat (length h))))
+        end
+    end.
+
+  Print stepsof.
+
+  Definition block_index (iindex : N) : N := block_index_impl program' iindex.
+
+  (* Helper function to get the total length (number of instructions) in the first n blocks of rrprog *)
+  Definition block_prefix_length (rrprog : list (list N)) (num_blocks : nat) : N:=
+    N.of_nat (List.fold_left (fun acc l => acc + (length l))%nat (firstn num_blocks rrprog) O).
+
+  (* True iff iindex is the index of a first instruction within a block output by r *)
+  Definition block_start (iindex : N) : Prop :=
+    (* Reasoning:
+       If the first n-1 blocks have |iindex| instructions then the instruction at iindex
+       is the first (0th) instruction of block n. *)
+    match N.compare (block_prefix_length program' (N.to_nat (N.pred (block_index iindex)))) iindex with
+    | Eq => True
+    | _ => False
+    end.
+  
+  Fixpoint reverse {A:Type} (l:list A) := List.fold_left (fun acc x => x::acc) l [].
+
+  Fixpoint flatten_1 {A:Type} (l:list (list A)) : list A :=
+    List.fold_left (fun acc l => acc ++ l) l [].
+
+  Definition code_prop (s : store) (code : list N) (base_addr:N) : Prop :=
+    (* Memory stores the program *)
+    xnbits (s V_MEM32) (base_addr * 8) ((4 * (N.of_nat (length code))) * 8) =
+      List.fold_left (fun acc insn => cbits acc 32 insn) (reverse code) 0
+    (* The program is executable *)
+    /\ xnbits (s A_EXEC) base_addr (4 * (N.of_nat (length code))) = N.ones (4 * (N.of_nat (length code)))
+    (* The program is not writeable *)
+    /\ xnbits (s A_WRITE) base_addr (4 * (N.of_nat (length code))) = 0.
+
+
+  (* I decided to make Pol take an `option id` instead of `id`. We can revisit this.
+     Reasoning: `label` is a partial function so it returns an option. Allowing Pol
+     to take an option and including the hypothesis that it is never true for 'None'
+     seemed like an easier interface for expressing the RPol definition rather than
+     adding another helper function or redirection. *)
+  Variable Pol : addr -> option id -> Prop.
+  Hypothesis PolNeverNone : forall a opt_id, Pol a opt_id -> exists id, opt_id = Some id.
+  Definition RPol (addr_from addr_to : addr) :=
+    Pol (block_index addr_from) (label (block_index addr_to)) /\ block_start addr_to (* policy-permitted jump *)
+      \/ block_index addr_from = block_index addr_to (* execution hasn't left the current block yet *)
+      \/ is_abort addr_to. (* jumps to "abort" are always safe *)
+
+  (* This wraps RPol, handling inputs of steps of traces of the form
+     (final exit-store pair, initial exit-store pair).
+
+     I'm undecided whether we should prove anything if either exit is
+     not an Addr - i.e. a hardware execution occurred. 
+
+     This could reasonably happen in a program, but with the proposed
+     CFG definition we cannot list any such jumps as OK because we
+     assume all jumps are from code to code.
+   *)
+  Definition RPolStep (xs_xs : ((exit * store) * (exit * store))) :=
+    match xs_xs with
+    | ((Addr addr_to,_), (Addr addr_from,_)) => RPol addr_from addr_to
+    | _ => True 
+    end.
+
+
+  (* For safety we only care that the trace respects the policy.
+     Below, in `correctness`, we'll prove that the rewritten program
+     behaves similarly to the original. *)
+  Definition safety :=
+    (*  t' - the trace of the executions of program and program' resp. 
+        s0' - the initial store of the executions.
+     *)
+    forall (t' : trace) (s0' : store) (xs' : prod exit store)
+    (RR: rr label policy program entry = Some program')
+    (* Both traces start at the entry *)
+    (ENTRY: startof t' xs' = (Addr entry, s0'))
+    (* Relate the program given as a list of instruction encodings with the initial store *)
+    (BIN: code_prop s0' (flatten_1 program') entry)
+    (* The trace represents a valid execution of the program *)
+    (EXEC: exec_prog p32_prog t'),
+      Forall RPolStep (stepsof t').
+
+  (*  An adaptation of the 1st part of Theorem 1 (page 204) from 
+      "Sound Transpilation from Binary to Machine-Independent Code"
+      by Metere et al. 
+
+      This states that all executions by the original either have a
+      corresponding execution that catches up to a similar end state
+      or aborts. *)
+  Definition original_has_simulation :=
+    (* program' is the rewritten program *)
+    forall (RR: rr label policy program entry = Some program'),
+    forall (t : trace) (s0 s0' : store) (xs : prod exit store)
+    (* Both traces start at the entry *)
+    (ENTRY: startof t xs = (Addr entry,s0))
+    (* Relate the program given as a list of instruction encodings with the initial store *)
+    (BIN: code_prop s0 program entry /\ code_prop s0' (flatten_1 program') entry)
+    (* The trace represents a valid execution of the program *)
+    (EXEC: exec_prog p32_prog t)
+    (* Assert the initial states are similar *)
+    (SIM: similar_states s0 s0')
+    (* The program has taken at least 1 step *)
+    (STEPS: (length t > 1)%nat),
+    (* There is a trace of the rewritten program that simulates the original or aborts *)
+      exists (t' : trace) (xs' : prod exit store), 
+         startof t' xs' = (Addr entry, s0') ->
+         exec_prog p32_prog t' ->
+         (length t' > 1)%nat 
+         /\ (is_aborted t' \/ match t, t' with 
+                              | (_,s)::_, (_,s')::_  => similar_states s s' 
+                              | _, _ => False 
+                              end).
+
+  (*  An adaptation of the second part (see above). 
+    
+      This states that all executions by the rewritten program that end at the
+      beginning of a rewritten block (corresponding to just before the execution
+      of the instruction) and have not aborted have a corresponding execution
+      of the original program that catchus up to them. *)
+  Definition rewritten_is_faithful :=
+    (* program' is the rewritten program *)
+    forall (RR: rr label policy program entry = Some program'),
+    (*  t,t' - the trace of the executions of program and program' resp. 
+        s0,s0' - the initial store of the executions.
+        xs,xs' - the "current" exit-store pair of the executions.
+     *)
+    forall (t' : trace) (s0 s0' s': store) (xs xs' : prod exit store) (a':addr)
+    (* Both traces start at the entry *)
+    (ENTRY: startof t' xs' = (Addr entry, s0'))
+    (* Relate the program given as a list of instruction encodings with the initial store *)
+    (BIN: code_prop s0 program entry /\ code_prop s0' (flatten_1 program') entry)
+    (* The trace represents a valid execution of the program *)
+    (EXEC': exec_prog p32_prog t')
+    (* Assert the initial states are similar *)
+    (SIM: similar_states s0 s0')
+    (STEPS': (length t' > 1)%nat)
+    (* Bind the latest state of t' to the start of a block. *)
+    (XS' : head t' = Some xs' /\ xs' = (Addr a', s'))
+    (START': match index_of_addr a' with Some n => block_start n | _ => False end)
+    (UNTERM': is_aborted t' -> False),
+      exists (t:trace), forall (a:addr) (s:store)
+      (START: startof t xs = (Addr entry,s0))
+      (STEPS: (length t > 1)%nat)
+      (END: head t = Some (Addr a, s)),
+      exec_prog p32_prog t /\ similar_states s s'.
+End RRCorrectness.
+
+Definition p32_rr label pol program entry :=
+  Some (rewrite_check_id label pol program entry).
+
+Theorem forall_stepsof_ind :
+  forall (X:Type) (P: X * X -> Prop)
+    (NIL: Forall P (stepsof nil))
+    (SINGLE: forall x, Forall P (stepsof [x]))
+    (IND: forall a h l (HEAD: P (a, h)) (TAIL: Forall P (stepsof (h::l))), Forall P (stepsof (a::h::l))),
+    forall l : list X, Forall P (stepsof l).
+Proof.
+  intros. induction l.
+  - apply Forall_nil.
+  - induction l.
+    -- apply SINGLE.
+    -- apply IND.
+       Check Forall_ind.
+
+(* Safety proof for our specific rewriter. *)
+Theorem p32_rr_safe :
+  forall program program' label policy entry is_abort (pol : addr -> option id -> Prop),
+    safety p32_rr label policy program entry program' is_abort pol.
+Proof.
+  unfold safety, exec_prog in *; intros. 
+  (* Would be nice to induct over `stepsof t'` so our inductive step has an
+     obvious last step, but we should also keep the relationship between the steps of t'
+     and t' starting at the entry obvious.
+
+     Maybe we should have a custom induction principle with 2 base cases - 
+     a base case for an empty trace, a base case for a singleton trace,
+     and then an induction step that works on a trace with at least one element
+     and proves the prop holds for traces with an additional (thus 2 total) specified
+     head element. *)
+  induction t'.
+
+  - apply Forall_nil.
+  - 
+Abort.
